theories/TM/L/UnfoldHeap.v
@@ -5,15 +5,303 @@ Require Import Undecidability.TM.Util.TM_facts.
 
 From Undecidability Require Import ProgrammingTools WriteValue Copy ListTM  JumpTargetTM WriteValue.
 From Undecidability.TM.L Require Import Alphabets LookupTM.
-From Undecidability.L.AbstractMachines.FlatPro Require Import LM_heap_def LM_heap_correct.
+From Undecidability.L.AbstractMachines.FlatPro Require Import LM_heap_def LM_heap_correct UnfoldHeap.
+From Undecidability.TM Require Import CaseList CasePair CaseCom CaseNat NatSub.
+
 From Undecidability Require Import L.L TM.TM.
-Require Import List.
-Import ListNotations.
+
 
 
 Import VectorNotations.
+Import ListNotations.
+Import Coq.Init.Datatypes List.
+
+Notation todo := (utils.todo).
+Open Scope string_scope.
+Require Import String.
+
+From Undecidability Require Cons_constant.
 
 Require Import Equations.Prop.DepElim.
+
+Module UnfoldClosStep.
+Section Fix.
+
+  Variable Σ : finType. 
+
+  Variable retr_stack : Retract (sigList (sigPair sigHClos sigNat)) Σ.
+  Variable retr_heap : Retract sigHeap Σ.
+
+  Definition retr_clos : Retract sigHClos Σ := ComposeRetract retr_stack _.
+
+  Definition retr_pro : Retract sigPro Σ := ComposeRetract retr_clos _.
+  Definition retr_com : Retract sigCom Σ := ComposeRetract retr_pro _.
+
+
+  Definition retr_nat_clos_ad' : Retract sigNat sigHClos := Retract_sigPair_X _ _.
+  Definition retr_nat_clos_ad : Retract sigNat Σ := ComposeRetract retr_clos retr_nat_clos_ad'.
+
+  Definition retr_nat_clos_var' : Retract sigNat sigHClos := Retract_sigPair_Y _ _.
+  Definition retr_nat_clos_var : Retract sigNat Σ := ComposeRetract retr_clos retr_nat_clos_var'.
+
+  Definition retr_stackEl : Retract (sigPair sigHClos sigNat) Σ :=
+    (ComposeRetract retr_stack _).
+
+  Definition retr_nat_stack : Retract sigNat Σ :=
+    ComposeRetract retr_stackEl
+            (Retract_sigPair_Y _ _) .
+
+  (** Instance of the [Lookup] and [JumpTarget] machine *)
+  Local Definition Lookup := Lookup retr_clos retr_heap.
+
+  Local Notation n := 20 (only parsing).
+
+  Local Notation i_a := Fin0 (only parsing).
+  Local Notation i_P := Fin1 (only parsing).
+  Local Notation i_k := Fin2 (only parsing).
+  Local Notation i_stack' := Fin3 (only parsing).
+  Local Notation i_res := Fin4 (only parsing).
+  Local Notation i_H := Fin5 (only parsing).
+  Local Notation i_aux1 := Fin6 (only parsing).
+  Local Notation i_aux2 := Fin7 (only parsing).
+  Local Notation i_aux3 := Fin8 (only parsing).
+  Local Notation i_aux4 := Fin9 (only parsing).
+
+  Definition Rel__step : pRel Σ^+ bool n :=
+    (fun t '(r, t') =>
+     forall (H : Heap) a P k stack' (res:Pro), 
+      t[@i_H] ≃(retr_heap) H
+      -> t[@i_a] ≃(retr_nat_clos_ad) a
+      -> t[@i_P] ≃(retr_pro) P
+      -> t[@i_k] ≃(retr_nat_clos_var) k
+      -> t[@i_stack'] ≃(retr_stack) stack'
+      -> t[@i_res] ≃(retr_pro) res
+      -> isRight t[@i_aux1]
+      -> isRight t[@i_aux2]
+      -> isRight t[@i_aux3]
+      -> isRight t[@i_aux4]
+      -> t'[@i_H] ≃(retr_heap) H
+      /\ isRight t'[@i_aux1] 
+      /\ isRight t'[@i_aux2] 
+      /\ isRight t'[@i_aux3] 
+      /\ isRight t'[@i_aux4]
+      /\ match unfoldTailRecStep H (((a,P),k)::stack',res) with
+            inr _ => False
+          | inl (stack2,res2) =>
+            t'[@i_res] ≃(retr_pro) res2 /\
+            match stack2 with
+            | [] =>
+              r = false
+              /\ isRight t'[@i_a]
+              /\ isRight t'[@i_P]
+              /\ isRight t'[@i_k]
+              /\ isRight t'[@i_stack']
+            | ((a2,P2),k2)::stack2' =>
+              r = true /\
+              t'[@i_a] ≃(retr_nat_clos_ad) a2
+              /\ t'[@i_P] ≃(retr_pro) P2
+              /\ t'[@i_k] ≃(retr_nat_clos_var) k2
+              /\ t'[@i_stack'] ≃(retr_stack) stack2'
+            end
+      end).
+
+    Arguments Rel__step : simpl never.
+
+    (* Print unfoldTailRecStep. *)
+    (*
+      Definition unfoldTailRecStep '(stack,res) : (list (HClos*nat) * Pro) + option Pro :=
+  match stack with
+    | ((a,P),k)::stack =>
+      match P with
+        c::P =>
+          match c with
+            varT n =>
+              if ( k <=? n)
+              then
+                  match lookup H a (n-k) with
+                  | Some (b,Q) =>
+                    inl (((b,Q),1)::(a,retT::P,S k)::stack,lamT::res)
+                  | None => inr None
+                  end
+              else
+                inl ((a,P,k)::stack,varT n::res)   
+          | appT => inl ((a,P,k)::stack,appT::res)         
+          | lamT => inl ((a,P,S k)::stack,lamT::res)
+          | retT => inl ((a,P,pred k)::stack,retT::res)
+          end
+        | [] => inl (stack,res)
+      end
+    | [] => inr (Some res)
+  end.
+  *)
+
+
+
+  Definition M__step : pTM (Σ) ^+ bool n :=
+    If
+      (CaseList _ ⇑ retr_pro @ [| i_P;i_aux1|]) 
+      (Switch (CaseCom ⇑ retr_com @ [|i_aux1|])
+        (fun i : option ACom=> match i with 
+          | Some c => 
+            Cons_constant.M (ACom2Com c)⇑ retr_pro @ [| i_res|];;
+            Return     
+            match c return match c with _ => _ end with
+            | retAT => (CaseNat ⇑ retr_nat_clos_var @ [|i_k|];;Return Nop tt)
+            | lamAT => Constr_S  ⇑ retr_nat_clos_var @ [|i_k|]
+            | appAT => Nop
+            end
+            true
+          | None (*var*) =>
+            CopyValue _  @ [| i_k;i_aux2|];;
+            CopyValue _  @ [| i_aux1;i_aux3|];;
+            If (Subtract ⇑ retr_nat_clos_var @ [|i_aux3;i_aux2|])
+               (Reset _ @ [|i_aux1|];;
+                CopyValue _  @ [| i_a;i_aux4|];;
+                If (Lookup @ [|i_H;i_aux4;i_aux3;i_aux1;i_aux2|])
+                  (Cons_constant.M lamT⇑ retr_pro @ [| i_res|];;
+                   Cons_constant.M retT⇑ retr_pro @ [| i_P|];;
+                   Constr_S  ⇑ retr_nat_clos_var @ [|i_k|];;
+                   Constr_pair _ _ ⇑ retr_clos @ [|i_a;i_P|];;
+                   Reset _ @ [|i_a|];;
+                   Translate retr_nat_clos_var retr_nat_stack @[|i_k|];;
+                   Constr_pair _ _ ⇑ retr_stackEl @ [|i_P;i_k|];;
+                   MoveValue _ @ [|i_aux1;i_P|];;
+                   Constr_cons _ ⇑ retr_stack @ [| i_stack';i_k|];;
+                   Reset _ @ [|i_k|];;
+                   CasePair _ _ ⇑ retr_clos @ [|i_P;i_a|];;
+                   Return (WriteValue (encode 1) ⇑ retr_nat_clos_var @ [|i_k|]) true 
+                  )
+                  (Return Diverge false)
+               )
+               (Return
+                 (Constr_varT ⇑ retr_com @ [|i_aux1|];;
+                  Constr_cons _ ⇑ retr_pro @ [| i_res;i_aux1|];;
+                  Reset _  @ [|i_aux1|];;
+                  Reset _ @ [|i_aux3|])
+                 true)
+        end)
+      )
+      ( Reset _ @ [|i_P|];;
+        Reset _ @ [|i_a|];;
+        Reset _ @ [|i_k|];;
+        If
+          (CaseList _ ⇑ retr_stack @ [| i_stack';i_k|])
+          (CasePair _ _ ⇑ retr_stackEl @ [|i_k;i_P|];;
+           CasePair _ _ ⇑ retr_clos @ [|i_P;i_a|];;
+           Translate retr_nat_stack retr_nat_clos_var @[|i_k|];;
+           Return Nop true
+          )
+          (Reset _ @ [|i_stack'|];;Return Nop false)
+      ).
+
+  Theorem Realise__step : Realise M__step Rel__step.
+  Proof.
+    eapply Realise_monotone.
+    {unfold M__step. TM_Correct_noSwitchAuto. TM_Correct.
+      1:now eapply RealiseIn_Realise, CaseCom_Sem. intros f.
+      destructBoth f.
+      {
+        TM_Correct. apply Cons_constant.Realise.
+         destructBoth a. all:TM_Correct.
+      }
+      TM_Correct.
+      all: (try (notypeclasses refine (@Reset_Realise _ _ _ _ _);shelve)).
+      all: try (notypeclasses refine (@CopyValue_Realise _ _ _ _ _);shelve).
+      now apply Subtract_Realise.
+      now apply Lookup_Realise.
+      1-2:now apply Cons_constant.Realise.
+      1,4:(notypeclasses refine (@Translate_Realise _  _ _ _ _ _);shelve).
+      now simple notypeclasses refine  (@MoveValue_Realise _ _ _ _ _ _ _ _ _);shelve.
+      now eapply RealiseIn_Realise, Constr_varT_Sem.
+    }
+    unfold Rel__step. hnf.
+    intros tin [y tout] Hif H a P k stack' res ? ? ? ? ? ?. destruct Hif as [Htrue | Hfalse]. 
+    - TMSimp. modpon H6. destruct P. easy. TMSimp.
+      modpon H7. destruct ymid as [ c | ].
+      + TMSimp. modpon H9. destruct c. all:TMSimp.
+        * modpon H14. destruct k,ymid. all:try contradiction. all:now simpl_surject.
+        * modpon H14. easy.    
+        * easy. 
+      + destruct H7 as (n&->&?). all:TMSimp. modpon H9;[]. modpon H14;[].
+        destruct H16. 
+        2:{
+          TMSimp. modpon H16;[]. modpon H19;[]. modpon H21;[]. modpon H23;[]. modpon H25;[].
+          replace (k <=? n) with false by easy. easy.
+        }
+        TMSimp. modpon H16;[]. modpon H18;[]. modpon H20;[].
+        replace (k <=? n) with true by easy.
+        destruct H22. 2:{ TMSimp;contradiction. }
+        TMSimp. modpon H22;[]. TMSimp.  modpon H24;[].  modpon H26;[].  modpon H28;[].  modpon H30.  modpon H32;[].
+        modpon H34;[]. modpon H36;[]. modpon H38;[]. modpon H40;[]. modpon H42;[].
+        modpon H44 ;[]. specialize (H47 1). modpon H47;[].
+        rename ymid into g.
+        replace (lookup H a (n - k)) with (Some g) by easy.
+        destruct g. easy.
+    - destruct Hfalse as (t0_ & Hfalse & t1_ & HRes1 & t2_ & HRes2 & t3_ & HRes3 & Hif).
+      TMSimp.      
+      modpon H12;[]. modpon H10;[]. modpon H6. 
+      destruct P. 2:contradiction.
+      TMSimp.
+      modpon H8.
+      destruct H13 as [Htrue | Hfalse]. all:TMSimp.
+      2:{
+        modpon H13. destruct stack'. 2:easy. TMSimp.
+        modpon H17. modpon H16. easy.
+      }
+      modpon H13;[]. destruct stack'. easy. TMSimp.
+      modpon H16;[]. TMSimp. modpon H18;[]. modpon H20;[].
+      easy.
+  Qed.                     
+
+
+End Fix.
+End UnfoldClosStep.
+
+Module UnfoldClos.
+Section Fix.
+
+  Variable Σ : finType.
+
+  Variable retr_clos : Retract sigHClos Σ.
+  Variable retr_heap : Retract sigHeap Σ.
+
+  (* Closure addresses *)
+
+  Definition retr_pro_clos : Retract sigPro sigHClos := _.
+  Local Definition retr_pro : Retract sigPro Σ := ComposeRetract retr_clos retr_pro_clos.
+  Local Definition retr_tok : Retract sigCom Σ := ComposeRetract retr_pro _.
+
+  Local Definition retr_nat_clos_ad : Retract sigNat sigHClos := Retract_sigPair_X _ (Retract_id _).
+  Local Definition retr_nat_step_clos_ad : Retract sigNat Σ := ComposeRetract retr_clos retr_nat_clos_ad.
+
+  Local Definition retr_nat_clos_var : Retract sigNat sigHClos := Retract_sigPair_Y _ _.
+  Local Definition retr_nat_step_clos_var : Retract sigNat Σ := ComposeRetract retr_clos retr_nat_clos_var.
+
+  (** Instance of the [Lookup] and [JumpTarget] machine *)
+  Local Definition Step_Lookup := Lookup retr_clos retr_heap.
+
+    Variable n : nat.
+
+    Variable i_g : Fin.t n.
+    Variable i_H : Fin.t n.
+    Variable o_t : Fin.t n.
+
+    Definition M : pTM (Σ) ^+ unit n. Admitted.
+
+    Theorem Realise :
+    Realise M (fun t '(r, t') =>
+                        forall g : HClos, forall H : Heap, 
+                            t[@i_g] ≃ g->
+                            t[@i_H] ≃ H ->
+                            exists t,
+                            reprC H g t /\
+                            t'[@o_t] ≃(retr_pro) compile t).
+    
+    Admitted.
+
+
+End Fix.
+End UnfoldClos.
 
 
 Module UnfoldHeap.
@@ -53,7 +341,7 @@ Section Fix.
 
     Definition M : pTM (Σ) ^+ unit n. Admitted.
 
-    Theorem Realises :
+    Theorem Realise :
     Realise M (fun t '(r, t') =>
                         forall g, forall H : Heap, 
                             t[@i_g] ≃(retr_closures_REMOVE) [g]%list (*TODO: change to clos?*) ->
